

Lista de Exercícios - Aula 10

Lista de Exercícios

$$1 - \binom{8}{3} = \frac{8!}{3!(8-3)!} = \frac{8 \cdot 7 \cdot 6 \cdot 5!}{3 \cdot 2 \cdot 1 \cdot 5!} = \frac{336}{6} = \boxed{56}$$

Alternativa B

$$2 - \binom{200}{198} = \frac{200!}{198!(200-198)!} = \frac{200 \cdot 199 \cdot 198!}{198! \cdot 2!} = \frac{39.800}{2} = \boxed{19.900}$$

Alternativa A

$$3 - \binom{n-1}{2} = \binom{n+1}{4} \rightarrow 1^o \text{ Caso: } \frac{(n-1)!}{2!(n-1-2)!} = \frac{(n+1)!}{4!(n+1-4)!}$$

$$\frac{(n-1)! \cdot 4! \cdot (n-3)!}{2! \cdot (n-3)!} = (n+1)n!$$

$$\frac{(n-1)! \cdot 4 \cdot 3 \cdot 2!}{2!} = (n+1)n \cdot (n-1)!$$

$$12 = \frac{(n^2+n) \cdot (n-1)!}{(n-1)!}$$

$$n^2 + n - 12 = 0$$

$$\frac{-4 \pm 3}{2} = \frac{-4 \pm 3}{2}$$

$$\frac{-4 + 3}{2} = \frac{-1}{2}$$

$$\frac{-4 - 3}{2} = \frac{-7}{2}$$

NÃO convém

convém
n = 3

$$2^o \text{ Caso: } \binom{n-1}{2} = \binom{n+1}{4} = 0 \rightarrow n < k$$

$$\begin{array}{l|l} n-1 < 2 & n+1 < 4 \\ n < 2+1 & n < 4-1 \\ \checkmark & \checkmark \\ n < 3 & n < 3 \\ \checkmark & \checkmark \\ n < 3 & \end{array}$$

$V = \{1, 2, 3\}$

$$4 - \binom{20}{13} + \binom{20}{14} = ? \quad \left| \begin{array}{l} \text{Soma de 2} \\ \text{consecutivos} \end{array} \right. > \binom{n}{k} + \binom{n}{k+1} = \binom{n+1}{k+1}$$

$$\hookrightarrow \binom{20}{13} + \binom{20}{14} = \binom{21}{14}$$

Alternativa C

★ Complementares: $\binom{n}{k} = \binom{n}{n-k}$

$$\binom{21}{14} = \binom{21}{21-14} = \binom{21}{7}$$

$$5 - \binom{n}{0} + \binom{n}{1} + \binom{n}{2} + \dots + \binom{n}{n} = 2^n \quad (\text{Soma na linha } n)$$

$$6-a) \sum_{p=0}^{10} \binom{10}{p} = \binom{10}{0} + \binom{10}{1} + \binom{10}{2} + \dots + \binom{10}{10} = 2^{10} = 1024$$

$$b) \sum_{p=0}^9 \binom{10}{p} = \binom{10}{0} + \binom{10}{1} + \binom{10}{2} + \dots + \binom{10}{9} = 2^{10} - \binom{10}{10} = 1024 - 1 = 1023$$

$$c) \sum_{p=2}^9 \binom{9}{p} = \binom{9}{2} + \binom{9}{3} + \dots + \binom{9}{9} = 2^9 - \binom{9}{1} - \binom{9}{0} = 512 - 9 - 1 = 502$$

$$d) \sum_{p=4}^{10} \binom{10}{p} = \binom{10}{4} + \binom{10}{5} + \dots + \binom{10}{10} = \binom{11}{5} \quad \rightarrow \text{Soma na coluna 4}$$

$$\binom{11}{5} = \frac{11!}{5! \cdot (11-5)!} = \frac{11 \cdot 10 \cdot 9 \cdot 8 \cdot 7 \cdot 6!}{5! \cdot 6!} = \frac{11 \cdot 10 \cdot 9 \cdot 8 \cdot 7}{5 \cdot 4 \cdot 3 \cdot 2 \cdot 1}$$

$$\hookrightarrow \frac{55440}{120} = 462$$

$$e) \sum_{p=5}^{10} \binom{p}{5} = \binom{5}{5} + \binom{6}{5} + \dots + \binom{10}{5} = \binom{11}{6} \rightarrow \text{Soma na coluna 5}$$

$$\hookrightarrow \binom{11}{6} = \frac{11!}{6!(11-5)!} = \frac{11 \cdot 10 \cdot 9 \cdot 8 \cdot 7 \cdot \cancel{6!}}{\cancel{6!} \cdot 5!} = \frac{11 \cdot 10 \cdot 9 \cdot 8 \cdot 7}{5 \cdot 4 \cdot 3 \cdot 2 \cdot 1}$$

$$\rightarrow \frac{55,440}{120} = 462_{\frac{1}{2}}$$

$$7 - \sum_{k=0}^m \binom{m}{k} = 512$$

$$\sum_{k=0}^m \binom{m}{k} = \binom{m}{0} + \dots + \binom{m}{m} = 512 \quad (\text{Soma na linha } m)$$

$$2^m = 512$$

$$2^m = 2^9$$

$$m = 9$$

→ Alternativa (e)